concurrency/concurrent_machine.v
@@ -48,6 +48,7 @@ Notation UNLOCK_SIG := (mksignature (AST.Tint::nil) (Some AST.Tint) cc_default).
 Notation UNLOCK := (EF_external "UNLOCK" UNLOCK_SIG).
 
 Notation block  := Values.block.
+
 Definition b_ofs2address b ofs : address:=
   (b, Int.intval ofs).
 
@@ -185,38 +186,6 @@ Module Type ThreadPoolSig.
       (Heq: j = latestThread tp)
       (cnt': containsThread (addThread tp vf arg pmap) j),
       getThreadR cnt' = pmap.
-
-  Axiom gsoAddRes:
-    forall {i tp} (cnt: containsThread tp i) vf arg pmap j
-      (cntj: containsThread tp j)
-      (cntj': containsThread (addThread tp vf arg pmap) j),
-      getThreadR cntj' = getThreadR cntj.
-
-  Axiom gssAddCode:
-    forall {i tp} (cnt: containsThread tp i) vf arg pmap j
-      (Heq: j = latestThread tp)
-      (cnt': containsThread (addThread tp vf arg pmap) j),
-      getThreadC cnt' = Kinit vf arg.
-
-  Axiom gsoAddCode:
-    forall {i tp} (cnt: containsThread tp i) vf arg pmap j
-      (cntj: containsThread tp j)
-      (cntj': containsThread (addThread tp vf arg pmap) j),
-      getThreadC cntj' = getThreadC cntj.
-
-  Axiom add_update_comm:
-    forall tp i vf arg pmap c' pmap'
-      (cnti: containsThread tp i)
-      (cnti': containsThread (addThread tp vf arg pmap) i),
-      addThread (updThread cnti c' pmap') vf arg pmap =
-      updThread cnti' c' pmap'.
-
-  Axiom add_updateC_comm:
-    forall tp i vf arg pmap c'
-      (cnti: containsThread tp i)
-      (cnti': containsThread (addThread tp vf arg pmap) i),
-      addThread (updThreadC cnti c') vf arg pmap =
-      updThreadC cnti' c'.
    
   (*Get thread Properties*)
   Axiom gssThreadCode :
